refocusing_examples/lam_ses_no_check.v
@@ -244,7 +244,7 @@ Module Lam_SES_NO_HandMachine <: ABSTRACT_MACHINE.
       end.
 
 
-  Definition next_conf0 (st : configuration) : option configuration :=
+  Definition dnext_conf (st : configuration) : option configuration :=
       match st with
 
       | [$ _, CBot, _, _ $]    => None
@@ -303,9 +303,9 @@ Module Lam_SES_NO_HandMachine <: ABSTRACT_MACHINE.
        | _ => None
        end. 
 
-  Definition next_conf (_ : entropy) := next_conf0.
+  Definition next_conf (_ : entropy) := dnext_conf.
 
-  Definition transition st1 st2 := next_conf0 st1 = Some st2.
+  Definition transition st1 st2 := dnext_conf st1 = Some st2.
 
 
   Instance rws : REWRITING_SYSTEM configuration :=
@@ -313,7 +313,7 @@ Module Lam_SES_NO_HandMachine <: ABSTRACT_MACHINE.
 
 
   Fact trans_computable0 :                              forall (st1 st2 : configuration),
-       `(rws) st1 → st2 <-> next_conf0 st1 = Some st2.
+       `(rws) st1 → st2 <-> dnext_conf st1 = Some st2.
 
   Proof. intuition. Qed.
 
@@ -330,8 +330,8 @@ Module Lam_SES_NO_HandMachine <: ABSTRACT_MACHINE.
 
 
 
-  Theorem next_conf0_eq_EAM :                                                  forall st,
-      next_conf0 st = Lam_SES_NO_EAM.next_conf0 st.
+  Theorem dnext_conf_eq_EAM :                                                  forall st,
+      dnext_conf st = Lam_SES_NO_EAM.dnext_conf st.
 
   Proof.
     destruct st as [[t k ? | k c v] ?].
@@ -344,7 +344,7 @@ Module Lam_SES_NO_HandMachine <: ABSTRACT_MACHINE.
   Corollary next_conf_eq_EAM :                                               forall e st,
       next_conf e st = Lam_SES_NO_EAM.next_conf e st.
 
-  Proof. eauto using next_conf0_eq_EAM. Qed.
+  Proof. eauto using dnext_conf_eq_EAM. Qed.
 
 
   Corollary transition_eqv_EAM :                                          forall st1 st2,
@@ -354,7 +354,7 @@ Module Lam_SES_NO_HandMachine <: ABSTRACT_MACHINE.
     intros.
     rewrite trans_computable, Lam_SES_NO_EAM.trans_computable.
     unfold Lam_SES_NO_EAM.next_conf, next_conf.
-    rewrite next_conf0_eq_EAM.
+    rewrite dnext_conf_eq_EAM.
     intuition.
   Qed.
 
