refocusing_examples/lam_ses_no_test.v
@@ -1,0 +1,38 @@
+Require Import Subset
+               abstract_machine_facts
+               lam_ses_no.
+
+Module Example.
+
+  Module Sim := DetAbstractMachine_Sim Lam_SES_NO_EAM.
+  Import Lam_SES_NO_EAM Lam_SES_NO_PreRefSem.
+
+
+  Definition t1 := Lam (App (Lam (Lam (Var 1))) (Var 0)).
+
+  Eval compute in 
+    Sim.n_steps 
+    ( load t1 )
+    17.
+
+
+  Fixpoint nat_term n :=
+    match n with
+    | 0   => Lam (Lam (Var 0))
+    | S n => Lam (Lam (App (Var 1) (App (App (nat_term n) (Var 1)) (Var 0))))
+    end.
+
+
+  Definition add_term := 
+      Lam (Lam (Lam (Lam 
+          (App (App (Var 3) 
+              (Var 1)) 
+              (App (App (Var 2) (Var 1)) (Var 0)))))).
+
+
+  Eval compute in
+      Sim.n_steps 
+      ( load (App (App add_term (nat_term 3)) (nat_term 4)) ) 
+      1890.
+
+End Example.
