rewriting_system/rewriting_system_following.v
@@ -8,7 +8,7 @@ Require Import Fin2
 Local Open Scope vector.
 
 Class RW_FOLLOWING                                    {configuration_er configuration_ed}
-    (Follower : REWRITING_SYSTEM configuration_er) 
+    (Follower : REWRITING_SYSTEM configuration_er)
     (Followed : REWRITING_SYSTEM configuration_ed) :=
 
 {
@@ -17,11 +17,11 @@ Class RW_FOLLOWING                                    {configuration_er configur
     semantics_surj : forall cd, exists cr, semantics cr = cd;
 
     correct :                                                             forall cr1 cr2,
-        `(Follower) cr1 → cr2  ->  semantics cr1 = semantics cr2  \/  
+        `(Follower) cr1 → cr2  ->  semantics cr1 = semantics cr2  \/
                                    `(Followed) semantics cr1 → semantics cr2;
 
     complete :                                                        forall cd1 cd2 cr1,
-        `(Followed) cd1 → cd2  ->  semantics cr1 = cd1 -> 
+        `(Followed) cd1 → cd2  ->  semantics cr1 = cd1 ->
             exists n (crs : Vector.t configuration_er n) cr2,
             (**)Forall (fun cr => semantics cr = cd1) crs /\
             (**)semantics cr2 = cd2                       /\
@@ -29,7 +29,7 @@ Class RW_FOLLOWING                                    {configuration_er configur
 
     no_silent_loops :
       ~ exists crs : nat -> configuration_er, (*a stream of configurations*)
-          forall n, 
-          (**)  `(Follower) crs n  →  crs (S n)  /\ 
+          forall n,
+          (**)  `(Follower) crs n  →  crs (S n)  /\
           (**)~ `(Followed) semantics (crs n)  →  semantics (crs (S n))
 }.
